aligned_alloc remaining lemmas
modular arithmetic lemma:
- n is a power of 2
- x and y are two divisors of n
- x <= y
then x divides y
(as x and y are powers of 2...)

lib_misc/MiscArith.fst
@@ -4,36 +4,6 @@ module MiscArith
 
 open FStar.Mul
 
-//TODO: to be removed
-//let mod_arith_lemma
-//  (n: nat) (k1 k2: pos)
-//  : Lemma
-//  (requires
-//    k1 % k2 == 0 /\
-//    k2 <= k1
-//  )
-//  (ensures
-//    (n % k1) % k2 == n % k2
-//  )
-//  =
-//  calc (==) {
-//    ((n / k1) * k1) % k2;
-//    == { Math.Lemmas.lemma_mod_mul_distr_r (n / k1) k1 k2 }
-//    ((n / k1) * (k1 % k2)) % k2;
-//    == { () }
-//    0;
-//  };
-//  assert (((n / k1) * k1) % k2 == 0);
-//  calc (==) {
-//    (n % k1) % k2;
-//    == { FStar.Math.Lemmas.euclidean_division_definition n k1 }
-//    (n - (n / k1) * k1) % k2;
-//    == { FStar.Math.Lemmas.lemma_mod_sub_distr n ((n / k1) * k1) k2 }
-//    (n - ((n / k1) * k1) % k2) % k2;
-//    == { () }
-//    n % k2;
-//  }
-
 let lemma_mod_plus2 (a k: int) (n: pos)
   : Lemma
   (requires
@@ -69,3 +39,221 @@ let lemma_div_le (a:pos) (b c k:nat)
   (requires k <= a * b * c)
   (ensures k / a <= b * c)
   = ()
+
+#push-options "--fuel 1 --ifuel 1"
+
+let rec decompose (n: pos)
+  : v:(nat & nat){(snd v) % 2 = 1}
+  = match n % 2 with
+  | 0 -> let (k1, k2) = decompose (n/2) in (k1+1, k2)
+  | 1 -> (0, n)
+
+open FStar.Mul
+let rec decompose_eq (n: pos)
+  : Lemma
+  (let (x,y) = decompose n in
+  n = (pow2 x) * y)
+  = match n % 2 with
+  | 0 -> decompose_eq (n/2)
+  | 1 -> ()
+
+#restart-solver
+
+open FStar.Math.Lemmas
+
+#push-options "--fuel 0 --ifuel 0 --z3rlimit 50 --split_queries always"
+let decompose_unicity_aux (i1 j1 i2 j2: nat)
+  : Lemma
+  (requires
+    (pow2 i1) * j1 == (pow2 i2) * j2 /\
+    j1 % 2 = 1 /\
+    j2 % 2 = 1 /\
+    j1 > 0 /\
+    j2 > 0 /\
+    i1 <= i2)
+  (ensures
+    i1 == i2
+  )
+  =
+  let t = j2 * (pow2 (i2 - i1)) in
+  calc (==) {
+    j1;
+    == { cancel_mul_div j1 (pow2 i1) }
+    j1 * (pow2 i1) / (pow2 i1);
+    == { swap_mul j1 (pow2 i1) }
+    (pow2 i2) * j2 / (pow2 i1);
+    == { swap_mul (pow2 i2) j2 }
+    j2 * (pow2 i2) / (pow2 i1);
+    == { pow2_plus (i2 - i1) i1 }
+    j2 * ((pow2 (i2 - i1)) * (pow2 i1)) / (pow2 i1);
+    == { paren_mul_right j2 (pow2 (i2 - i1)) (pow2 i1) }
+    t * (pow2 i1) / (pow2 i1);
+    == { cancel_mul_div t (pow2 i1) }
+    t;
+  };
+  if (i2 > i1) then (
+    let k = pow2 (i2 - i1) in
+    assert (j1 == j2 * k);
+    assert_norm (k % 2 = 0);
+    lemma_mod_mul2 j2 k 2;
+    assert ((k * j2) % 2 = 0);
+    assert (j1 % 2 = 0);
+    assert (j1 % 2 = 1)
+  )
+#pop-options
+
+let decompose_unicity (n: pos) (i1 j1 i2 j2:nat)
+  : Lemma
+  (requires
+    n = (pow2 i1) * j1 /\
+    n = (pow2 i2) * j2 /\
+    j1 % 2 = 1 /\
+    j2 % 2 = 1 /\
+    i1 >= 0 /\
+    i2 >= 0 /\
+    j1 > 0 /\
+    j2 > 0
+  )
+  (ensures
+    i1 = i2 /\ j1 = j2
+  )
+  (decreases n)
+  =
+  if (i1 = i2) then () else (
+    assert ((pow2 i1) * j1 == (pow2 i2) * j2);
+    if (i1 < i2)
+    then decompose_unicity_aux i1 j1 i2 j2
+    else decompose_unicity_aux i2 j2 i1 j1
+  )
+
+let mul_abcd_acbd (a b c d: nat)
+  : Lemma
+  ((a * b) * (c * d) == (a * c) * (b * d))
+  = ()
+
+let mul_odd_odd_is_odd (a b: nat)
+  : Lemma
+  (requires a % 2 = 1 /\ b % 2 = 1)
+  (ensures (a * b) % 2 = 1)
+  =
+  lemma_mod_mul_distr_l a b 2
+
+let decompose_mul (n1 n2: pos)
+  : Lemma
+  (let i0, j0 = decompose (n1 * n2) in
+  let i1, j1 = decompose n1 in
+  let i2, j2 = decompose n2 in
+  (i0 = i1 + i2) /\
+  (j0 = j1 * j2))
+  =
+  let i0, j0 = decompose (n1 * n2) in
+  decompose_eq (n1 * n2);
+  let i1, j1 = decompose n1 in
+  let i2, j2 = decompose n2 in
+  calc (==) {
+    n1 * n2;
+    == { decompose_eq n1 }
+    ((pow2 i1) * j1) * n2;
+    == { decompose_eq n2 }
+    ((pow2 i1) * j1) * ((pow2 i2) * j2);
+    == { mul_abcd_acbd (pow2 i1) j1 (pow2 i2) j2 }
+    ((pow2 i1) * (pow2 i2)) * (j1 * j2);
+    == { pow2_plus i1 i2 }
+    (pow2 (i1 + i2)) * (j1 * j2);
+  };
+  assert (n1 * n2 = (pow2 (i1 + i2)) * (j1 * j2));
+  mul_odd_odd_is_odd j1 j2;
+  decompose_unicity (n1 * n2) i0 j0 (i1+i2) (j1*j2)
+
+let decompose_pow2 (k: nat)
+  : Lemma
+  (decompose (pow2 k) = (k, 1))
+  =
+  let (x,y) = decompose (pow2 k) in
+  decompose_eq (pow2 k);
+  decompose_unicity (pow2 k) k 1 x y
+
+let rec mod_thm (k: nat) (n: pos)
+  : Lemma
+  (requires
+    n <= pow2 k /\
+    (pow2 k) % n = 0
+  )
+  (ensures (
+    let (x,y) = decompose n in
+    y = 1
+  ))
+  = match (decompose n) with
+  | (0, y) ->
+      let z = pow2 k in
+      euclidean_division_definition z n;
+      assert (z = z/n * n);
+      (* LHS decomposition *)
+      decompose_pow2 k;
+      assert (decompose (pow2 k) = (k, 1));
+      (* RHS decomposition *)
+      let i1, j1 = decompose (z/n) in
+      decompose_mul (z/n) n;
+      assert (decompose (z/n * n) == (i1 + 0, j1 * y));
+      (* eq *)
+      assert (k = i1 + 0 /\ 1 = j1 * y)
+  | (x, y) ->
+      let a = pow2 (k-1) in
+      let b = 2 in
+      let c = n/2 in
+      calc (==) {
+        (pow2 k) % n;
+        == { pow2_plus (k-1) 1 }
+        (a * b) % n;
+        == { () }
+        (a * b) % (b * c);
+        == { Math.Lemmas.modulo_scale_lemma a b c }
+        (a % c) * b;
+      };
+      mod_thm (k-1) (n/2)
+
+let rec pow2_mod (k1 k2: nat)
+  : Lemma
+  (requires k1 <= k2)
+  (ensures (pow2 k2) % (pow2 k1) == 0)
+  (decreases k1)
+  = match k1 with
+  | 0 -> ()
+  | _ ->
+      pow2_plus (k2 - 1) 1;
+      pow2_plus 1 (k1 - 1);
+      Math.Lemmas.modulo_scale_lemma (pow2 (k2 - 1)) 2 (pow2 (k1 - 1));
+      assert ((pow2 k2) % (pow2 k1) == ((pow2 (k2 - 1)) % (pow2 (k1 - 1))) * 2);
+      pow2_mod (k1 - 1) (k2 - 1)
+
+let pow2_is_increasing (x y: nat)
+  : Lemma
+  (requires pow2 x <= pow2 y)
+  (ensures x <= y)
+  =
+  if x > y then
+  pow2_lt_compat x y
+
+let alignment_lemma (v:nat) (n: nat) (x y: pos)
+  : Lemma
+  (requires
+    v = pow2 n /\
+    v % x == 0 /\
+    v % y == 0 /\
+    x <= v /\
+    y <= v /\
+    x <= y)
+  (ensures
+    y % x == 0
+  )
+  =
+  let (i1, j1) = decompose x in
+  let (i2, j2) = decompose y in
+  mod_thm n x;
+  mod_thm n y;
+  assert (j1 == 1 /\ j2 == 1);
+  decompose_eq x;
+  decompose_eq y;
+  pow2_is_increasing i1 i2;
+  assert (i1 <= i2);
+  pow2_mod i1 i2
